

Zatihan 3 :

No _____
Date _____

1. Diketahui :

$$A = \begin{bmatrix} 3 & -1 \\ 2 & 4 \end{bmatrix}$$

$$B = \begin{bmatrix} 0 & 2 \\ 1 & -4 \end{bmatrix}$$

$$C = \begin{bmatrix} 4 & 1 \\ -3 & -2 \end{bmatrix}$$

$$a = 4 \\ b = -7$$

Buktikanlah :

a/ $a(BC) = (aB)C = B(aC)$

Jwb

$$4 \left(\begin{bmatrix} 0 & 2 \\ 1 & -4 \end{bmatrix} \begin{bmatrix} 4 & 1 \\ -3 & -2 \end{bmatrix} \right) = 4 \left(\begin{bmatrix} 0 & 2 \\ 1 & -4 \end{bmatrix} \right) \begin{bmatrix} 4 & 1 \\ -3 & -2 \end{bmatrix} = \begin{bmatrix} 0 & 2 \\ 1 & -4 \end{bmatrix} \left(4 \begin{bmatrix} 4 & 1 \\ -3 & -2 \end{bmatrix} \right)$$

$$4 \begin{bmatrix} -6 & -4 \\ 16 & 9 \end{bmatrix} = \begin{bmatrix} 0 & 8 \\ 4 & -16 \end{bmatrix} \begin{bmatrix} 4 & 1 \\ -3 & -2 \end{bmatrix} = \begin{bmatrix} 0 & 2 \\ 1 & -4 \end{bmatrix} \begin{bmatrix} 16 & 4 \\ -12 & -8 \end{bmatrix}$$

$$\begin{bmatrix} -24 & -16 \\ 64 & 36 \end{bmatrix} = \begin{bmatrix} -24 & -16 \\ 64 & 36 \end{bmatrix} = \begin{bmatrix} -24 & -16 \\ 64 & 36 \end{bmatrix} //$$

b/ $A(B-C) = AB - AC$

Jwb

$$\begin{bmatrix} 3 & -1 \\ 2 & 4 \end{bmatrix} \left(\begin{bmatrix} 0 & 2 \\ 1 & -4 \end{bmatrix} - \begin{bmatrix} 4 & 1 \\ -3 & -2 \end{bmatrix} \right) = \begin{bmatrix} 3 & -1 \\ 2 & 4 \end{bmatrix} \begin{bmatrix} 0 & 2 \\ 1 & -4 \end{bmatrix} - \begin{bmatrix} 3 & -1 \\ 2 & 4 \end{bmatrix} \begin{bmatrix} 4 & 1 \\ -3 & -2 \end{bmatrix}$$

$$= \begin{bmatrix} 3 & -1 \\ 2 & 4 \end{bmatrix} \begin{bmatrix} -4 & 1 \\ 4 & -2 \end{bmatrix} = \begin{bmatrix} -1 & 10 \\ 4 & -12 \end{bmatrix} - \begin{bmatrix} 15 & 5 \\ -4 & -6 \end{bmatrix}$$

$$= \begin{bmatrix} -16 & 5 \\ 8 & -6 \end{bmatrix} = \begin{bmatrix} -16 & 5 \\ 8 & -6 \end{bmatrix} //$$

c/ $(A^T)^T = A$

Jwb

$$\left(\begin{bmatrix} 3 & -1 \\ 2 & 4 \end{bmatrix}^T \right)^T = \begin{bmatrix} 3 & -1 \\ 2 & 4 \end{bmatrix}$$

$$= \begin{bmatrix} 3 & 2 \\ -1 & 4 \end{bmatrix}^T = \begin{bmatrix} 3 & -1 \\ 2 & 4 \end{bmatrix}$$

$$= \begin{bmatrix} 3 & -1 \\ 2 & 4 \end{bmatrix} = \begin{bmatrix} 3 & -1 \\ 2 & 4 \end{bmatrix} //$$

$$d_1 (AB)^T = B^T A^T$$

Jwb

$$\left(\begin{bmatrix} 3 & -1 \\ 2 & 4 \end{bmatrix} \begin{bmatrix} 0 & 2 \\ 1 & -4 \end{bmatrix} \right)^T = \begin{bmatrix} 0 & 2 \\ 1 & -4 \end{bmatrix}^T \begin{bmatrix} 3 & -1 \\ 2 & 4 \end{bmatrix}^T$$

$$= \begin{bmatrix} -1 & 10 \\ 4 & -12 \end{bmatrix}^T = \begin{bmatrix} 0 & 1 \\ 2 & -4 \end{bmatrix} \begin{bmatrix} 3 & 2 \\ -1 & 4 \end{bmatrix}$$

$$= \begin{bmatrix} -1 & 4 \\ 10 & -12 \end{bmatrix} = \begin{bmatrix} -1 & 4 \\ 10 & -12 \end{bmatrix} //$$

$$e_1 (aC)^T = aC^T$$

Jwb

$$\left(4 \begin{bmatrix} 4 & 1 \\ -3 & -2 \end{bmatrix} \right)^T = 4 \begin{bmatrix} 4 & 1 \\ -3 & -2 \end{bmatrix}^T$$

$$= \begin{bmatrix} 16 & 4 \\ -12 & -8 \end{bmatrix}^T = 4 \begin{bmatrix} 4 & -3 \\ 1 & -2 \end{bmatrix}$$

$$= \begin{bmatrix} 16 & -12 \\ 4 & -8 \end{bmatrix} = \begin{bmatrix} 16 & -12 \\ 4 & -8 \end{bmatrix} //$$

2. carilah invers dari matriks berikut :

a. $A = \begin{bmatrix} 2 & -3 \\ 4 & 4 \end{bmatrix}$

Jwb $A^{-1} = \frac{1}{20} \begin{bmatrix} 4 & 3 \\ -4 & 2 \end{bmatrix}$

$$A^{-1} = \begin{bmatrix} \frac{4}{20} & \frac{3}{20} \\ \frac{-4}{20} & \frac{2}{20} \end{bmatrix} = \begin{bmatrix} \frac{1}{5} & \frac{3}{20} \\ -\frac{1}{5} & \frac{1}{10} \end{bmatrix} //$$

b. $B = \begin{bmatrix} 3 & 1 \\ 5 & 2 \end{bmatrix}$

Jwb $B^{-1} = \frac{1}{1} \begin{bmatrix} 2 & -1 \\ -5 & 3 \end{bmatrix}$

$$B^{-1} = \begin{bmatrix} 2 & -1 \\ -5 & 3 \end{bmatrix} //$$

c. $C = \begin{bmatrix} 2 & 0 \\ 0 & 3 \end{bmatrix}$

Jwb $C^{-1} = \frac{1}{6} \begin{bmatrix} 3 & 0 \\ 0 & 2 \end{bmatrix}$

$$C^{-1} = \begin{bmatrix} \frac{3}{6} & 0 \\ 0 & \frac{2}{6} \end{bmatrix} = \begin{bmatrix} \frac{1}{2} & 0 \\ 0 & \frac{1}{3} \end{bmatrix} //$$

d. $D = \begin{bmatrix} 6 & 4 \\ -2 & -1 \end{bmatrix}$

Jwb $D^{-1} = \frac{1}{2} \begin{bmatrix} -1 & -4 \\ 2 & 6 \end{bmatrix}$

$$= \begin{bmatrix} -\frac{1}{2} & -\frac{4}{2} \\ \frac{2}{2} & \frac{6}{2} \end{bmatrix} = \begin{bmatrix} -\frac{1}{2} & -2 \\ 1 & 3 \end{bmatrix} //$$

Berdasarkan matriks diatas, buktikanlah :

$$e, (A^T)^{-1} = (A^{-1})^T$$

Jwb

$$\left(\begin{bmatrix} 2 & -3 \\ 4 & 4 \end{bmatrix}^T \right)^{-1} = \left(\begin{bmatrix} 2 & -3 \\ 4 & 4 \end{bmatrix}^{-1} \right)^T$$

$$= \begin{bmatrix} 2 & 4 \\ -3 & 4 \end{bmatrix}^{-1} = \left(\frac{1}{8 - (-12)} \begin{bmatrix} 4 & 3 \\ -4 & 2 \end{bmatrix} \right)^T$$

$$= \frac{1}{20} \begin{bmatrix} 4 & -4 \\ 3 & 2 \end{bmatrix} = \left(\frac{1}{20} \begin{bmatrix} 4 & 3 \\ -4 & 2 \end{bmatrix} \right)^T$$

$$= \begin{bmatrix} \frac{4}{20} & \frac{-4}{20} \\ \frac{3}{20} & \frac{2}{20} \end{bmatrix} = \begin{bmatrix} \frac{4}{20} & \frac{3}{20} \\ \frac{-4}{20} & \frac{2}{20} \end{bmatrix}^T$$

$$= \begin{bmatrix} \frac{4}{20} & \frac{-4}{20} \\ \frac{3}{20} & \frac{2}{20} \end{bmatrix} = \begin{bmatrix} \frac{4}{20} & \frac{-4}{20} \\ \frac{3}{20} & \frac{2}{20} \end{bmatrix} //$$

$$f, (ABC)^T = C^T B^T A^T$$

Jwb

$$\left(\begin{bmatrix} 2 & -3 \\ 4 & 4 \end{bmatrix} \begin{bmatrix} 3 & 1 \\ 5 & 2 \end{bmatrix} \begin{bmatrix} 2 & 0 \\ 0 & 3 \end{bmatrix} \right)^T = \begin{bmatrix} 2 & 0 \\ 0 & 3 \end{bmatrix}^T \begin{bmatrix} 3 & 1 \\ 5 & 2 \end{bmatrix}^T \begin{bmatrix} 2 & -3 \\ 4 & 4 \end{bmatrix}^T$$

$$= \left(\begin{bmatrix} -9 & -4 \\ 32 & 12 \end{bmatrix} \begin{bmatrix} 2 & 0 \\ 0 & 3 \end{bmatrix} \right)^T = \begin{bmatrix} 2 & 0 \\ 0 & 3 \end{bmatrix} \begin{bmatrix} 3 & 5 \\ 1 & 2 \end{bmatrix} \begin{bmatrix} 2 & 4 \\ -3 & 4 \end{bmatrix}$$

$$= \begin{bmatrix} -18 & -12 \\ 64 & 36 \end{bmatrix}^T = \begin{bmatrix} 6 & 10 \\ 3 & 6 \end{bmatrix} \begin{bmatrix} 2 & 4 \\ -3 & 4 \end{bmatrix}$$

$$= \begin{bmatrix} -18 & 64 \\ -12 & 36 \end{bmatrix} = \begin{bmatrix} -18 & 64 \\ -12 & 36 \end{bmatrix} //$$

$$g, (ABC)^{-1} = C^{-1} B^{-1} A^{-1}$$

Jwb

$$\left(\begin{bmatrix} 2 & -3 \\ 4 & 4 \end{bmatrix} \begin{bmatrix} 3 & 1 \\ 5 & 2 \end{bmatrix} \begin{bmatrix} 2 & 0 \\ 0 & 3 \end{bmatrix} \right)^{-1} = \begin{bmatrix} 2 & 0 \\ 0 & 3 \end{bmatrix}^{-1} \begin{bmatrix} 3 & 1 \\ 5 & 2 \end{bmatrix}^{-1} \begin{bmatrix} 2 & -3 \\ 4 & 4 \end{bmatrix}^{-1}$$

$$= \left(\begin{bmatrix} -9 & -4 \\ 32 & 12 \end{bmatrix} \begin{bmatrix} 2 & 0 \\ 0 & 3 \end{bmatrix} \right)^{-1} = \frac{1}{6} \begin{bmatrix} 3 & 0 \\ 0 & 2 \end{bmatrix} \frac{1}{1} \begin{bmatrix} 2 & -1 \\ -5 & 3 \end{bmatrix} \frac{1}{20} \begin{bmatrix} 4 & 3 \\ -4 & 2 \end{bmatrix}$$

$$= \left(\begin{bmatrix} -18 & -12 \\ 64 & 36 \end{bmatrix} \right)^{-1} = \begin{bmatrix} \frac{3}{6} & 0 \\ 0 & \frac{2}{6} \end{bmatrix} \begin{bmatrix} 2 & -1 \\ -5 & 3 \end{bmatrix} \begin{bmatrix} \frac{4}{20} & \frac{3}{20} \\ \frac{-4}{20} & \frac{2}{20} \end{bmatrix}$$

$$= \frac{1}{120} \begin{bmatrix} 36 & 12 \\ -64 & -18 \end{bmatrix} = \begin{bmatrix} \frac{6}{6} & \frac{-3}{6} \\ \frac{-10}{6} & \frac{6}{6} \end{bmatrix} \begin{bmatrix} \frac{4}{20} & \frac{3}{20} \\ \frac{-4}{20} & \frac{2}{20} \end{bmatrix}$$

$$= \begin{bmatrix} \frac{36}{120} & \frac{12}{120} \\ \frac{-64}{120} & \frac{-18}{120} \end{bmatrix} = \begin{bmatrix} 1 & -\frac{1}{2} \\ -\frac{5}{3} & 1 \end{bmatrix} \begin{bmatrix} \frac{1}{5} & \frac{3}{20} \\ -\frac{1}{5} & \frac{1}{10} \end{bmatrix}$$

$$= \begin{bmatrix} \frac{2+1}{10} & \frac{2}{20} \\ \frac{-5-3}{18} & \frac{-18+6}{60} \end{bmatrix}$$

$$\begin{bmatrix} \frac{36}{120} & \frac{12}{120} \\ \frac{-64}{120} & \frac{-18}{120} \end{bmatrix} = \begin{bmatrix} \frac{3 \times 12}{10} & \frac{2 \times 6}{20} \\ \frac{-8 \times 8}{18} & \frac{-9 \times 2}{60} \end{bmatrix}$$

$$= \begin{bmatrix} \frac{36}{120} & \frac{12}{120} \\ \frac{-64}{120} & \frac{-18}{120} \end{bmatrix} = \begin{bmatrix} \frac{36}{120} & \frac{12}{120} \\ \frac{-64}{120} & \frac{-18}{120} \end{bmatrix} //$$

3. Temukanlah A :

$$a_1 (7A)^{-1} = \begin{bmatrix} -3 & 7 \\ 1 & -2 \end{bmatrix}$$

Jawab

$$(7A)^{-1} = 7^{-1} \cdot A^{-1} = \begin{bmatrix} -3 & 7 \\ 1 & -2 \end{bmatrix}$$

$$= \frac{1}{7} \cdot A^{-1} = \begin{bmatrix} -3 & 7 \\ 1 & -2 \end{bmatrix}$$

$$A^{-1} = 7 \begin{bmatrix} -3 & 7 \\ 1 & -2 \end{bmatrix}$$

$$A^{-1} = \begin{bmatrix} -21 & 49 \\ 7 & -14 \end{bmatrix}$$

$$A = -\frac{1}{49} \begin{bmatrix} -14 & -49 \\ -7 & -21 \end{bmatrix} = \begin{bmatrix} \frac{14}{49} & \frac{49}{49} \\ \frac{7}{49} & \frac{21}{49} \end{bmatrix}$$

$$= \begin{bmatrix} \frac{2}{7} & 1 \\ \frac{1}{7} & \frac{3}{7} \end{bmatrix} //$$

$$b, (5A^T)^{-1} = \begin{bmatrix} -3 & -1 \\ 5 & 2 \end{bmatrix}$$

Jwb

$$(5A^T)^{-1} = 5^{-1} \cdot (A^T)^{-1} = \begin{bmatrix} -3 & -1 \\ 5 & 2 \end{bmatrix}$$

$$= \frac{1}{5} (A^T)^{-1} = \begin{bmatrix} -3 & -1 \\ 5 & 2 \end{bmatrix}$$

$$(A^T)^{-1} = 5 \begin{bmatrix} -3 & -1 \\ 5 & 2 \end{bmatrix}$$

$$(A^T)^{-1} = \begin{bmatrix} -15 & -5 \\ 25 & 10 \end{bmatrix}$$

$$A^{-1} = \begin{bmatrix} -15 & 25 \\ -5 & 10 \end{bmatrix}$$

$$A = -\frac{1}{25} \begin{bmatrix} 10 & -25 \\ 5 & -15 \end{bmatrix}$$

$$= \begin{bmatrix} \frac{-10}{25} & \frac{25}{25} \\ \frac{-5}{25} & \frac{15}{25} \end{bmatrix}$$

$$A = \begin{bmatrix} \frac{-2}{5} & 1 \\ \frac{-1}{5} & \frac{3}{5} \end{bmatrix} //$$

4. Diketahui :

$$A = \begin{bmatrix} 3 & 1 \\ 2 & 1 \end{bmatrix}$$

$$B = \begin{bmatrix} 2 & 0 \\ 4 & 1 \end{bmatrix}$$

a. A^3

Jwb

$$\begin{bmatrix} 3 & 1 \\ 2 & 1 \end{bmatrix} \begin{bmatrix} 3 & 1 \\ 2 & 1 \end{bmatrix} \begin{bmatrix} 3 & 1 \\ 2 & 1 \end{bmatrix} = \begin{bmatrix} 11 & 4 \\ 8 & 3 \end{bmatrix} \begin{bmatrix} 3 & 1 \\ 2 & 1 \end{bmatrix}$$

$$A^3 = \begin{bmatrix} 41 & 15 \\ 30 & 11 \end{bmatrix} //$$

b. B^3

Jwb

$$\begin{bmatrix} 2 & 0 \\ 4 & 1 \end{bmatrix} \begin{bmatrix} 2 & 0 \\ 4 & 1 \end{bmatrix} \begin{bmatrix} 2 & 0 \\ 4 & 1 \end{bmatrix} = \begin{bmatrix} 4 & 0 \\ 12 & 1 \end{bmatrix} \begin{bmatrix} 2 & 0 \\ 4 & 1 \end{bmatrix}$$

$$B^3 = \begin{bmatrix} 8 & 0 \\ 28 & 1 \end{bmatrix} //$$

c. A^{-3}

Jwb

$$\begin{bmatrix} 3 & 1 \\ 2 & 1 \end{bmatrix}^{-1} \begin{bmatrix} 3 & 1 \\ 2 & 1 \end{bmatrix}^{-1} \begin{bmatrix} 3 & 1 \\ 2 & 1 \end{bmatrix}^{-1} = \frac{1}{1} \begin{bmatrix} 1 & -1 \\ -2 & 3 \end{bmatrix} \begin{bmatrix} 1 & -1 \\ -2 & 3 \end{bmatrix} \begin{bmatrix} 1 & -1 \\ -2 & 3 \end{bmatrix}$$

$$= \begin{bmatrix} 1 & -1 \\ -2 & 3 \end{bmatrix} \begin{bmatrix} 1 & -1 \\ -2 & 3 \end{bmatrix} \begin{bmatrix} 1 & -1 \\ -2 & 3 \end{bmatrix}$$

$$= \begin{bmatrix} 3 & -4 \\ -8 & 11 \end{bmatrix} \begin{bmatrix} 1 & -1 \\ -2 & 3 \end{bmatrix}$$

$$= \begin{bmatrix} 11 & -15 \\ -30 & 41 \end{bmatrix} ///$$

$$d, B^{-3}$$

jawab

$$\begin{aligned} \begin{bmatrix} 2 & 0 \\ 4 & 1 \end{bmatrix}^{-1} \begin{bmatrix} 2 & 0 \\ 4 & 1 \end{bmatrix}^{-1} \begin{bmatrix} 2 & 0 \\ 4 & 1 \end{bmatrix}^{-1} &= \frac{1}{2} \begin{bmatrix} 1 & 0 \\ -4 & 2 \end{bmatrix} \cdot \frac{1}{2} \begin{bmatrix} 1 & 0 \\ -4 & 2 \end{bmatrix} \cdot \frac{1}{2} \begin{bmatrix} 1 & 0 \\ -4 & 2 \end{bmatrix} \\ &= \begin{bmatrix} \frac{1}{2} & 0 \\ -2 & 1 \end{bmatrix} \begin{bmatrix} \frac{1}{2} & 0 \\ -2 & 1 \end{bmatrix} \begin{bmatrix} \frac{1}{2} & 0 \\ -2 & 1 \end{bmatrix} \\ &= \begin{bmatrix} \frac{1}{4} & 0 \\ -3 & 1 \end{bmatrix} \begin{bmatrix} \frac{1}{2} & 0 \\ -2 & 1 \end{bmatrix} \\ &= \begin{bmatrix} \frac{1}{8} & 0 \\ -\frac{7}{2} & 1 \end{bmatrix} // \end{aligned}$$

$$e, A^2 - 2A + I$$

jawab

$$\begin{aligned} \begin{bmatrix} 3 & 1 \\ 2 & 1 \end{bmatrix} \begin{bmatrix} 3 & 1 \\ 2 & 1 \end{bmatrix} - 2 \begin{bmatrix} 3 & 1 \\ 2 & 1 \end{bmatrix} + \begin{bmatrix} 1 & 0 \\ 0 & 1 \end{bmatrix} \\ = \begin{bmatrix} 11 & 4 \\ 8 & 3 \end{bmatrix} - \begin{bmatrix} 6 & 2 \\ 4 & 2 \end{bmatrix} + \begin{bmatrix} 1 & 0 \\ 0 & 1 \end{bmatrix} \\ = \begin{bmatrix} 6 & 2 \\ 4 & 2 \end{bmatrix} // \end{aligned}$$

$$f, B^2 - 2B + I$$

jawab

$$\begin{aligned} \begin{bmatrix} 2 & 0 \\ 4 & 1 \end{bmatrix} \begin{bmatrix} 2 & 0 \\ 4 & 1 \end{bmatrix} - 2 \begin{bmatrix} 2 & 0 \\ 4 & 1 \end{bmatrix} + \begin{bmatrix} 1 & 0 \\ 0 & 1 \end{bmatrix} \\ = \begin{bmatrix} 4 & 0 \\ 12 & 1 \end{bmatrix} - \begin{bmatrix} 4 & 0 \\ 8 & 2 \end{bmatrix} + \begin{bmatrix} 1 & 0 \\ 0 & 1 \end{bmatrix} = \begin{bmatrix} 1 & 0 \\ 4 & 0 \end{bmatrix} // \end{aligned}$$